rocq/rules.v
@@ -22,7 +22,7 @@ Definition update_simple (stt: Stt) (so: simple_outcome) : Stt :=
         let ce := curendurance stt in
             update_endurance (fun e => Nat.min me (ce + me / 2))%nat stt
     | GainItem i q => update_items (add_item i q) stt
-    | LoseItem i q => update_items (rm_item i q) stt
+    | LoseItem i q => c_rm_items i q stt
     | LoseItemKind slts => update_items (fun items => fold_right lose_all_slot items slts) stt
     | MustEat ch =>
         match (ch, s_check Hunting (disciplines stt)) with
@@ -30,11 +30,11 @@ Definition update_simple (stt: Stt) (so: simple_outcome) : Stt :=
         | _ =>
             let b01ls := Nat.eqb (book stt) 1
              in if b01ls && (Nat.ltb 3 (max_hp stt - curendurance stt)) && has_item Laumspur stt
-              then update_items (rm_item Laumspur 1) (heal stt 3)
+              then c_rm_items Laumspur 1 (heal stt 3)
               else if has_item Meal stt
-                    then update_items (rm_item Meal 1) stt
+                    then c_rm_items Meal 1 stt
                     else if b01ls && has_item Laumspur stt
-                          then update_items (rm_item Laumspur 1) (heal stt 3)
+                          then c_rm_items Laumspur 1 (heal stt 3)
                           else update_endurance (fun e => e - 3)%nat stt
         end
     | StoreEquipment => 
@@ -176,7 +176,7 @@ Fixpoint lose_items (s: slot) (q: nat) (stt: Stt): Proba Stt :=
         match losable with
         | [] => certain stt
         | _ => let withoutitem := fun i: item => 
-                let nstt := update_items (rm_item i 1) stt in
+                let nstt := c_rm_items i 1 stt in
                     (Q2Qc (1 / inject_Z (Z.of_nat amnt)), lose_items s nq nstt)
                 in
           merge_probas (map withoutitem losable)
@@ -295,7 +295,7 @@ Inductive WellFormedCO: chapter_outcome -> Prop :=
   .
 
 Inductive WellFormedDecision: decision -> Prop :=
-  | check_decisions: forall decs, Forall WellFormedDecision decs -> (exists d, In d decs) -> WellFormedDecision (Decisions decs)
+  | check_decisions: forall d1 d2, WellFormedDecision d1 -> WellFormedDecision d2 -> WellFormedDecision (App d1 d2)
   | check_retrieve_equipment: forall d, WellFormedDecision d -> WellFormedDecision (retrieve_equipment d)
   | check_can_take: forall i q d, (q > 0)%nat -> WellFormedDecision d -> WellFormedDecision (can_take i q d)
   | check_can_buy: forall i q d, (q > 0)%nat -> WellFormedDecision d -> WellFormedDecision (can_buy i q d)
@@ -470,7 +470,7 @@ Module RHelpers.
   Qed.
 
   Fixpoint dec_amount (nitems_cost: nat) (d: decision): nat := match d with
-  | Decisions lst => 1 + list_sum (map (dec_amount nitems_cost) lst)
+  | App d1 d2 => 1 + dec_amount nitems_cost d1 + dec_amount nitems_cost d2
   | retrieve_equipment nxt => 
     1 + nitems_cost + dec_amount 0 nxt
   | can_take _ q nxt => 1 + q + dec_amount nitems_cost nxt
@@ -494,18 +494,169 @@ Module RHelpers.
   | MustDrop : list item -> can_take_result
   .
 
-  Definition tcan_take (i: item) (q: nat) (s: Stt): can_take_result :=
+  Definition tcan_take (i: item) (s: Stt): can_take_result :=
     match item_slot i with
     | SSpecial | SPouch => SpaceAvailable
     | SWeapon =>
         let weapons := all_character_items_slot s SWeapon in
         let amount := list_sum (map snd weapons) in
-        if amount <? 2 then SpaceAvailable else MustDrop (map fst weapons)
+        if amount <? 2 then SpaceAvailable else MustDrop (map fst (filter (fun iq : item * nat => (0 <? snd iq)%nat && (negb (mps.eqb i (fst iq)))) weapons))
     | SBackpack =>
         let bpis := all_character_items_slot s SBackpack in
         let amount := list_sum (map snd bpis) in
-        if amount <? 8 then SpaceAvailable else MustDrop (map fst bpis)
+        if amount <? 8 then SpaceAvailable else MustDrop (map fst (filter (fun iq : item * nat => (0 <? snd iq)%nat && (negb (mps.eqb i (fst iq))))  bpis))
     end.
+
+  Lemma tcan_take_notin: forall i s lst, tcan_take i s = MustDrop lst ->
+    ~ In i lst.
+  Proof.
+    intros. intro contra.
+    unfold tcan_take in H.
+    destruct (item_slot i) eqn: SLOT; try discriminate.
+    * destruct (list_sum (map snd (all_character_items_slot s SWeapon)) <? 2); try discriminate.
+      remember (map fst (filter (fun iq : item * nat => (0 <? snd iq) && negb (mps.eqb i (fst iq))) (all_character_items_slot s SWeapon))).
+      inversion H; subst; clear H.
+      apply in_map_fst in contra.
+      destruct contra.
+      apply filter_In in H.
+      destruct H.
+      apply andb_true_iff in H0.
+      destruct H0.
+      apply negb_true_iff in H1.
+      apply eqb_not in H1.
+      simpl in H1.
+      contradiction.
+    * destruct (list_sum (map snd (all_character_items_slot s SBackpack)) <? 8); try discriminate.
+      remember (map fst (filter (fun iq : item * nat => (0 <? snd iq) && negb (mps.eqb i (fst iq))) (all_character_items_slot s SBackpack))).
+      inversion H; subst; clear H.
+      apply in_map_fst in contra.
+      destruct contra.
+      apply filter_In in H.
+      destruct H.
+      apply andb_true_iff in H0.
+      destruct H0.
+      apply negb_true_iff in H1.
+      apply eqb_not in H1.
+      simpl in H1.
+      contradiction.
+  Qed.
+
+  Lemma tcan_take_slot: forall i s lst, tcan_take i s = MustDrop lst ->
+    Forall (fun e => item_slot e = item_slot i) lst.
+  Proof.
+    intros.
+    unfold tcan_take in H.
+    destruct (item_slot i) eqn: SLOT; try discriminate.
+    * destruct (list_sum (map snd (all_character_items_slot s SWeapon)) <? 2); try discriminate.
+      remember (map fst (filter (fun iq : item * nat => (0 <? snd iq) && negb (mps.eqb i (fst iq))) (all_character_items_slot s SWeapon))).
+      inversion H; subst; clear H.
+      apply Forall_forall.
+      intros.
+      apply in_map_fst in H.
+      destruct H.
+      apply filter_In in H.
+      destruct H. unfold all_character_items_slot in H.
+      apply filter_In in H.
+      destruct H.
+      simpl in *.
+      apply mps.eqb_correct in H1.
+      exact H1.
+    * destruct (list_sum (map snd (all_character_items_slot s SBackpack)) <? 8); try discriminate.
+      remember (map fst (filter (fun iq : item * nat => (0 <? snd iq) && negb (mps.eqb i (fst iq))) (all_character_items_slot s SBackpack))).
+      inversion H; subst; clear H.
+      eapply Forall_forall.
+      intros.
+      apply in_map_fst in H.
+      destruct H.
+      apply filter_In in H.
+      destruct H. unfold all_character_items_slot in H.
+      apply filter_In in H.
+      destruct H.
+      simpl in *.
+      apply mps.eqb_correct in H1.
+      exact H1.
+  Qed.
+
+  Lemma lookup_helper_found: forall i sl s q,
+    ValidMap (items s) ->
+    item_slot i = sl ->
+    lookup i (all_character_items_slot s sl) = Some q <-> lookup i (items s) = Some q.
+  Proof.
+    intros i sl s q VMM IS.
+    unfold all_character_items_slot.
+    split; intro MH.
+    * apply vmap_in in MH. 2: {apply Slot.valid. auto. }
+      apply filter_In in MH.
+      destruct MH as [P1 P2].
+      apply vmap_in in P1; auto.
+    * apply vmap_in.
+      apply Slot.valid. auto.
+      apply filter_In.
+      simpl.
+      split.
+      + apply vmap_in; auto.
+      + apply mps.eqb_correct in IS.
+        exact IS.
+  Qed.
+
+  Lemma tcan_take_in: forall i s lst, ValidMap (items s) -> tcan_take i s = MustDrop lst ->
+    forall drp,
+      In drp lst ->
+      i <> drp /\ (sitems drp s > 0)%nat.
+  Proof.
+    intros i s lst VSS.
+    intros.
+    split. {
+      intro contra.
+      subst.
+      pose proof (tcan_take_notin _ _ _ H).
+      contradiction.
+    }
+    unfold tcan_take in H.
+    destruct (item_slot i) eqn: SLOT; try discriminate.
+    * destruct (list_sum (map snd (all_character_items_slot s SWeapon)) <? 2); try discriminate.
+      inversion H;subst;clear H.
+      unfold all_character_items_slot in H0.
+      apply in_map_iff in H0.
+      destruct H0 as [x [A B]].
+      destruct x as [ni nq].
+      simpl in *.
+      subst.
+      apply filter_In in B.
+      destruct B as [B C].
+      simpl in C.
+      apply filter_In in B.
+      destruct B as [B D].
+      simpl in *.
+      unfold sitems.
+      apply vmap_in in B; auto.
+      rewrite B.
+      apply andb_true_iff in C.
+      destruct C.
+      apply Nat.ltb_lt in H.
+      Lia.lia.
+    * destruct (list_sum (map snd (all_character_items_slot s SBackpack)) <? 8); try discriminate.
+      inversion H;subst;clear H.
+      unfold all_character_items_slot in H0.
+      apply in_map_iff in H0.
+      destruct H0 as [x [A B]].
+      destruct x as [ni nq].
+      simpl in *.
+      subst.
+      apply filter_In in B.
+      destruct B as [B C].
+      simpl in C.
+      apply filter_In in B.
+      destruct B as [B D].
+      simpl in *.
+      unfold sitems.
+      apply vmap_in in B; auto.
+      rewrite B.
+      apply andb_true_iff in C.
+      destruct C.
+      apply Nat.ltb_lt in H.
+      Lia.lia.
+  Qed.
 
   Definition simplify_retrieve_equipment (stt: Stt) (nxt: decision) :=
       let takable := previtems stt in
@@ -518,6 +669,75 @@ Module RHelpers.
   
   Definition item_cost (stt: Stt)  : nat := list_sum (map snd (previtems stt)) + length (previtems stt).
 
+  Lemma update_stt_preserve_cost:
+      forall stt f, (previtems stt = previtems (f stt)) -> item_cost (f stt) = item_cost stt.
+  Proof.
+    intros.
+    unfold item_cost.
+    rewrite !H.
+    reflexivity.
+  Qed.
+
+  Definition add_rm (stt: Stt) (add rm: item) :=
+    update_items (add_item add 1) (c_rm_items rm 1 stt).
+
+  Lemma add_rm_preserve_cost:
+      forall stt add rm, item_cost (add_rm stt add rm) = item_cost stt.
+  Proof.
+    intros.
+    destruct stt. unfold item_cost. simpl. reflexivity.
+  Qed.
+
+  Lemma add_rm_preserve_count:
+      forall stt add rm sl,
+       ValidBag (items stt) ->
+       item_slot add = item_slot rm ->
+       add <> rm ->
+       (sitems rm stt > 0)%nat ->
+       all_character_items_slot_count (add_rm stt add rm) sl = all_character_items_slot_count stt sl.
+  Proof.
+    intros stt add rm sl VMM Hslot Hdiff Hhasrm.
+    unfold add_rm.
+    pose proof (Slot.add_rm stt add rm VMM Hdiff Hslot Hhasrm sl).
+    unfold all_character_items_slot_count, update_items, update_endurance in *; simpl in *.
+    unfold sitems, add_item in *. simpl in *.
+    assumption.
+  Qed.
+
+  Lemma add_rm_preserve: forall stt add rm i,
+    ValidMap (items stt) ->
+    has_item i stt = true -> rm <> i -> has_item i (add_rm stt add rm) = true.
+  Proof.
+    intros.
+    unfold has_item, add_rm, c_rm_items, has, rm_item, bag_rm in *.
+    simpl.
+    destruct (eq_dec add Gold).
+    * subst. rewrite add_item_gold.
+      destruct (eq_dec i Gold).
+      + subst.
+        rewrite Lookup.lookup_insert_with.
+        rewrite Lookup.update_diff; auto.
+        destruct (lookup Gold (items stt)); auto.
+        destruct (n + 1 <? 51) eqn: X;auto.
+        destruct n; simpl; auto.
+        apply Update.valid; auto.
+      + rewrite Lookup.lookup_insert_with_diff; auto.
+        rewrite Lookup.update_diff; auto.
+        apply Update.valid; auto.
+      + Lia.lia.
+    * rewrite add_item_nogold; auto.
+      destruct (eq_dec i add).
+      + subst.
+        rewrite Lookup.lookup_insert_with.
+        rewrite Lookup.update_diff; auto.
+        destruct (lookup add (items stt)); auto.
+        destruct n0; simpl; auto.
+        apply Update.valid; auto.
+      + rewrite Lookup.lookup_insert_with_diff; auto.
+        rewrite Lookup.update_diff; auto.
+        apply Update.valid; auto.
+  Qed.
+
   Lemma update_items_preserve_cost:
       forall stt f, item_cost (update_items f stt) = item_cost stt.
   Proof.
@@ -525,9 +745,255 @@ Module RHelpers.
     destruct stt. unfold item_cost. simpl. reflexivity.
   Qed.
 
+  Program Definition mk_updated_add_rm (stt : Stt) (add rm: item)
+    : {nstt | RHelpers.item_cost (add_rm stt add rm) = RHelpers.item_cost stt} :=
+  exist _ (add_rm stt add rm) (add_rm_preserve_cost stt add rm).
+
   Program Definition mk_updated_item (stt : Stt) (f: Items -> Items)
     : {nstt | RHelpers.item_cost (update_items f stt) = RHelpers.item_cost stt} :=
   exist _ (update_items f stt) (update_items_preserve_cost stt f).
+
+  Program Definition mk_updated_stt (stt : Stt) (f: Stt -> Stt) (H: forall stt, previtems stt = previtems (f stt))
+    : {nstt | RHelpers.item_cost (f stt) = RHelpers.item_cost stt} :=
+  exist _ (f stt) (update_stt_preserve_cost stt f (H stt)).
+
+  Program Definition get_wtakestts (stt: Stt) (i: item) : 
+  list {nstt | RHelpers.item_cost nstt = RHelpers.item_cost stt } :=
+  match RHelpers.tcan_take i stt with
+  | RHelpers.SpaceAvailable => [mk_updated_item stt (add_item i 1)]
+  | RHelpers.MustDrop lst => 
+      map (fun drp => RHelpers.mk_updated_add_rm stt i drp : {nstt | RHelpers.item_cost nstt = RHelpers.item_cost stt}) lst
+  end.
+
+  Lemma get_wtakestts_valid: forall stt i out nstt, ValidState stt ->
+     out = get_wtakestts stt i -> In nstt out ->
+     ValidState (proj1_sig nstt).
+  Proof.
+    intros stt i out nstt VSS Eqout IO.
+    destruct (tcan_take i stt) eqn: tct.
+    { (* space available *)
+      unfold get_wtakestts in Eqout. simpl in *. subst.
+      rewrite tct in IO.
+      destruct nstt; simpl in *. destruct IO; try contradiction.
+      inversion H; subst; clear H.
+      unfold ValidState, ValidBag in *.
+      simpl in *.
+      {
+      repeat split; try tauto.
+        * destruct stt; simpl in *. unfold update_items in *; simpl.
+          unfold sitems. simpl.
+          destruct (eq_dec Gold i).
+          + subst. rewrite add_item_gold; auto.
+            rewrite Lookup.lookup_insert_with; try tauto.
+            destruct (lookup Gold items) eqn: G.
+            - destruct (n + 1 <? 51) eqn:LT; auto.
+              apply Nat.ltb_lt in LT. Lia.lia.
+            - Lia.lia.
+          + rewrite add_item_nogold; auto.
+            rewrite Lookup.lookup_insert_with_diff; try tauto.
+        * unfold tcan_take in tct.
+          destruct (item_slot i) eqn: SLOT.
+          + rewrite Slot.no_increase; try tauto. unfold ValidBag. tauto.
+            intro contra.
+            rewrite SLOT in contra.
+            discriminate.
+          + rewrite Slot.increase; auto; try tauto. 
+            destruct (list_sum (map snd (all_character_items_slot stt SBackpack)) <? 8) eqn: LT.
+            apply Nat.ltb_lt in LT. unfold all_character_items_slot_count.
+            simpl. simpl in LT. Lia.lia.
+            discriminate.
+            intro contra.
+            subst.
+            discriminate.
+          + rewrite Slot.no_increase; try (unfold ValidBag; tauto). rewrite SLOT. intro contra. discriminate.
+          + rewrite Slot.no_increase; try (unfold ValidBag; tauto). rewrite SLOT. intro contra. discriminate.
+        * unfold tcan_take in tct.
+          destruct (item_slot i) eqn: SLOT.
+          + rewrite Slot.increase; auto; try tauto. 
+            destruct (list_sum (map snd (all_character_items_slot stt SWeapon)) <? 2) eqn: LT.
+            apply Nat.ltb_lt in LT. unfold all_character_items_slot_count.
+            simpl. simpl in LT. Lia.lia.
+            discriminate.
+            intro contra.
+            subst.
+            discriminate.
+          + rewrite Slot.no_increase; try (unfold ValidBag; tauto). rewrite SLOT. intro contra. discriminate.
+          + rewrite Slot.no_increase; try (unfold ValidBag; tauto). rewrite SLOT. intro contra. discriminate.
+          + rewrite Slot.no_increase; try (unfold ValidBag; tauto). rewrite SLOT. intro contra. discriminate.
+        * unfold add_item. destruct i; apply Insert.insert_with_valid; tauto.
+        * destruct (eq_dec Gold i).
+          + unfold add_item. subst. 
+            apply Forall_forall.
+            intros.
+            destruct x.
+            simpl in *.
+            apply Nat.eqb_neq.
+            intro contra.
+            subst.
+            apply vmap_in in H. 2: {
+              apply Insert.insert_with_valid.
+              tauto.
+            }
+            destruct (eq_dec i Gold).
+            - subst.
+              rewrite Lookup.lookup_insert_with in H.
+              destruct (lookup Gold (items stt)) eqn: GLD.
+              ** destruct (n + 1 <? 51); simpl in H. inversion H.
+                 Lia.lia.
+                inversion H.
+              ** inversion H.
+              ** tauto.
+            - rewrite Lookup.lookup_insert_with_diff in H; auto; try tauto.
+              apply vmap_in in H; try tauto.
+              destruct VSS as [A [B [C [D [E [F [G [[I1 I2] [J [K L]]]]]]]]]].
+              eapply Forall_forall in I2; eauto.
+              simpl in I2.
+              discriminate.
+          + rewrite add_item_nogold; auto.
+            apply add_valid_no_zero; auto.
+            unfold ValidBag.
+            tauto.
+        * assert (max_hp stt <= max_hp (update_items (add_item i 1) stt))%nat as MHP. {
+            apply (VS.max_hp_add_items stt i 1); try tauto.
+            Lia.lia.
+          }
+          Lia.lia.
+      }
+    }
+    { (* must drop *)
+    unfold get_wtakestts in Eqout. simpl in *. subst.
+    pose proof (tcan_take_notin i stt l tct) as NI.
+    rewrite tct in IO.
+    apply in_map_iff in IO.
+    destruct IO as [drp [Heq Hin]].
+    inversion Heq; subst. simpl. clear H.
+    unfold ValidState in *.
+    simpl in *.
+    repeat (split; try tauto).
+    + unfold max_hp.
+      apply Nat.min_glb_lt; try Lia.lia.
+      assert (0 < maxendurance (update_items (rm_item drp 1) stt))%nat. {
+        unfold update_items.
+        simpl.
+        Lia.lia.
+      }
+      Lia.lia.
+    + unfold sitems, add_rm, update_items; simpl.
+      destruct (eq_dec i Gold).
+      - subst.
+        rewrite add_item_gold; auto.
+        rewrite Lookup.lookup_insert_with.
+        destruct (eq_dec drp Gold).
+        subst. contradiction.
+        unfold rm_item, bag_rm.
+        rewrite Lookup.update_diff; auto.
+        -- destruct (lookup Gold (items stt)).
+           destruct (n0 + 1 <? 51) eqn: L51.
+           apply Nat.ltb_lt in L51.
+           Lia.lia.
+           Lia.lia.
+           Lia.lia.
+        -- unfold ValidBag in VSS. tauto.
+        -- pose proof (rm_valid (items stt) drp 1).
+           lapply H. intros. destruct H0. tauto. tauto.
+      - rewrite add_item_nogold; auto.
+        rewrite Lookup.lookup_insert_with_diff; auto.
+        destruct (eq_dec Gold drp).
+        --  subst. unfold rm_item, bag_rm.
+            rewrite Lookup.update_eq_b; auto; try tauto.
+            destruct (lookup Gold (items stt)) eqn: GLD; try Lia.lia.
+            destruct n0; simpl; auto. Lia.lia.
+            destruct n0; simpl; auto. Lia.lia.
+            unfold sitems in VSS. rewrite GLD in VSS. Lia.lia.
+            unfold ValidBag in VSS.
+            tauto.
+        -- unfold rm_item, bag_rm.
+           unfold ValidBag, sitems in VSS.
+           rewrite Lookup.update_diff; auto; tauto.
+        -- unfold rm_item.
+           apply Update.valid.
+           unfold ValidBag in VSS.
+           tauto.
+    + rewrite add_rm_preserve_count; try tauto.
+      - apply tcan_take_slot in tct.
+        eapply Forall_forall in tct; eauto.
+      - intro contra. subst. contradiction.
+      - epose proof (tcan_take_in _ _ _ _ tct _ Hin). tauto.
+        Unshelve. unfold ValidBag in VSS. tauto.
+    + rewrite add_rm_preserve_count; try tauto.
+      - apply tcan_take_slot in tct.
+        eapply Forall_forall in tct; eauto.
+      - intro contra. subst. contradiction.
+      - epose proof (tcan_take_in _ _ _ _ tct _ Hin). tauto.
+        Unshelve. unfold ValidBag in VSS. tauto.
+    + destruct (eq_dec i Gold).
+      - subst. simpl.
+        apply Insert.insert_with_valid.
+        unfold rm_item.
+        unfold bag_rm.
+        apply Update.valid.
+        unfold ValidBag in VSS.
+        tauto.
+      - rewrite add_item_nogold;auto.
+        apply Insert.insert_with_valid.
+        unfold rm_item.
+        unfold bag_rm.
+        apply Update.valid.
+        unfold ValidBag in VSS.
+        tauto.
+    + apply Forall_forall.
+      intros.
+      destruct x as [itm q].
+      simpl.
+      apply Nat.eqb_neq.
+      intro contra.
+      subst.
+      apply vmap_in in H. 2: {
+        apply add_item_valid_bag. Lia.lia.
+        apply rm_valid.
+        tauto.
+      }
+      apply lookup_cant_be_zero in H; auto.
+      apply add_item_valid_bag. Lia.lia.
+      apply rm_valid.
+      tauto.
+    + assert (ValidMap (items (update_items (rm_item drp 1) stt))) as CND. {
+        unfold update_items, rm_item, bag_rm.
+        simpl.
+        apply Update.valid. unfold ValidBag in VSS.
+        tauto.
+      }
+      pose proof (VS.has_item_kept (update_items (rm_item drp 1) stt) BodyArmor i 1 CND) as BA.
+      pose proof (VS.has_item_kept (update_items (rm_item drp 1) stt) Helmet i 1 CND) as HE.
+      unfold add_rm, c_rm_items, update_items, max_hp, has_item in *.
+      simpl in *.
+      remember (rm_item drp 1 (items stt)) as rstt.
+      assert ((if has Helmet (add_item i 1 rstt) then 2 else 0) <= 2)%nat. {
+        destruct (has Helmet (add_item i 1 rstt)); Lia.lia.
+      }
+      assert ((if has BodyArmor (add_item i 1 rstt) then 4 else 0) <= 4)%nat. {
+        destruct (has BodyArmor (add_item i 1 rstt)); Lia.lia.
+      }
+      { destruct (has BodyArmor rstt) eqn: PBA.
+      * lapply BA; auto.
+        clear BA; intro BA.
+        rewrite BA.
+        destruct (has Helmet rstt) eqn: PHE.
+        + lapply HE; auto.
+          clear HE; intro HE.
+          rewrite HE.
+          pose proof (Nat.le_min_r (curendurance stt) (maxendurance stt + 4 + 2)).
+          Lia.lia.
+        + Lia.lia.
+      * destruct (has Helmet rstt) eqn: PHE; try Lia.lia.
+        lapply HE; auto.
+        clear HE; intro HE.
+        rewrite HE.
+        Lia.lia.
+      }
+    }
+  Qed.
+
 End RHelpers.
 
 Section FlattenDec.
@@ -536,35 +1002,25 @@ Ltac fd_solver := match goal with
   | |- RHelpers.item_cost (update_items _ ?stt) = RHelpers.item_cost ?stt => 
         apply RHelpers.update_items_preserve_cost
   | nstt : {_ | RHelpers.item_cost _ = RHelpers.item_cost _} |- _ => destruct nstt; simpl in *
-  | |- (forall _ : list decision, Decisions _ <> ?w) /\ _ => unfold w; repeat (split; intros; try (intro contra; inversion contra))
   | |- _ => Lia.lia
   end.
 
 Local Obligation Tactic := intros; subst; simpl; repeat fd_solver.
 
-Program Fixpoint flatten_decision (stt: Stt) (d: decision) {measure (RHelpers.dec_amount (RHelpers.item_cost stt) d)}
-  : list (Proba next_step) :=
-  match d with
-    | can_take i q nxt =>
-      let notake := flatten_decision stt nxt in
-      let wtakestts : list {nstt | RHelpers.item_cost nstt = RHelpers.item_cost stt } := match RHelpers.tcan_take i q stt with
-                    | RHelpers.SpaceAvailable => [RHelpers.mk_updated_item stt (add_item i 1)]
-                    | RHelpers.MustDrop lst => map (fun drp => RHelpers.mk_updated_item stt
-                            (fun ns => rm_item drp 1 (add_item i 1 ns)) :
-                             {nstt | RHelpers.item_cost nstt = RHelpers.item_cost stt}) lst
-                    end in
-      match q with
-      | 0%nat => [] (* can't happen *)
-      | 1%nat => notake ++ flat_map (fun nstt => flatten_decision (proj1_sig nstt) nxt) wtakestts
-      | S q => notake ++ flat_map (fun nstt => flatten_decision (proj1_sig nstt) (can_take i q nxt)) wtakestts
-      end
-    | Decisions lst =>
-      match lst with
-      | [] => []
-      | [d] => flatten_decision stt d
-      | d::ds => flatten_decision stt d ++ flatten_decision stt (Decisions ds)
-      end
-    | retrieve_equipment nxt =>
+Equations flatten_decision (stt: Stt) (d: decision) : list (Proba next_step) 
+  by wf (RHelpers.dec_amount (RHelpers.item_cost stt) d) lt :=
+flatten_decision stt (can_take _ 0 _) := []; (* can't happen *)
+flatten_decision stt (can_take i 1 nxt) :=
+  let notake := flatten_decision stt nxt in
+  let wtakestts := RHelpers.get_wtakestts stt i in
+     notake ++ flat_map (fun nstt => flatten_decision (proj1_sig nstt) nxt) wtakestts;
+flatten_decision stt (can_take i (S (S q'')) nxt) :=
+  let q' := S q'' in
+  let notake := flatten_decision stt nxt in
+  let wtakestts := RHelpers.get_wtakestts stt i in
+    notake ++ flat_map (fun nstt => flatten_decision (proj1_sig nstt) (can_take i q' nxt)) wtakestts;
+flatten_decision stt (App d1 d2) := flatten_decision stt d1 ++ flatten_decision stt d2;
+flatten_decision stt (retrieve_equipment nxt) :=
     let nstt := {| book := book stt
                   ; maxendurance := maxendurance stt
                   ; curendurance := curendurance stt
@@ -576,153 +1032,254 @@ Program Fixpoint flatten_decision (stt: Stt) (d: decision) {measure (RHelpers.de
                   ; previtems := empty
                   |} in
     let ndecision := RHelpers.simplify_retrieve_equipment stt nxt in
-        flatten_decision nstt ndecision
-    | _ => []
-  end.
-Next Obligation.
-rewrite e. Lia.lia.
-Defined.
-Next Obligation.
-rewrite e. Lia.lia.
-Defined.
-Next Obligation.
-  remember (list_sum (map (RHelpers.dec_amount (RHelpers.item_cost stt)) ds)) as x.
-  pose proof (RHelpers.dec_amount_positive (RHelpers.item_cost stt) d).
-  Lia.lia.
-Defined.
-Next Obligation.
-intro contra. 
-unfold ds in *. inversion contra.
-Defined.
+        flatten_decision nstt ndecision;
+flatten_decision stt (can_buy i cost nxt) :=
+  let notake := flatten_decision stt nxt in
+  let pstt: Stt := c_rm_items Gold cost stt in
+  let wtakestts := RHelpers.get_wtakestts pstt i in
+    if cost <? sitems Gold stt
+      then notake ++ flat_map (fun nstt => flatten_decision (proj1_sig nstt) nxt) wtakestts
+      else notake;
+flatten_decision stt _ := []
+.
 Next Obligation.
 unfold ndecision.
-unfold RHelpers.item_cost.
-destruct stt. simpl in *.
-unfold RHelpers.simplify_retrieve_equipment in *.
-simpl in *.
-clear nstt flatten_decision ndecision flags items chapter disciplines sk maxendurance curendurance book.
-induction previtems.
-* simpl.  Lia.lia.
-* destruct a. simpl. destruct (0 <? n); simpl; Lia.lia.
+unfold RHelpers.simplify_retrieve_equipment.
+unfold nstt.
+clear ndecision nstt.
+destruct stt; simpl in *.
+unfold RHelpers.item_cost. simpl.
+clear flatten_decision flags items chapter disciplines sk maxendurance curendurance book.
+induction previtems; simpl; try Lia.lia.
+destruct a.
+destruct (0 <? n); simpl; Lia.lia.
 Defined.
 Next Obligation.
-apply measure_wf.
-apply lt_wf.
+rewrite e.
+Lia.lia.
 Defined.
-End FlattenDec.
+Next Obligation.
+rewrite e.
+Lia.lia.
+Defined.
+Next Obligation.
+rewrite e.
+subst pstt.
+assert (RHelpers.item_cost (c_rm_items Gold cost stt) = RHelpers.item_cost stt). {
+  apply RHelpers.update_stt_preserve_cost.
+  destruct stt.
+  reflexivity.
+}
+rewrite H.
+Lia.lia.
+Defined.
 
-Module FDH.
-  Lemma flatten_decision_cons: forall d ds stt, flatten_decision stt (Decisions (d::ds)) =
-        flatten_decision stt d ++ flatten_decision stt (Decisions ds).
-  Proof.
-    intros.
-  Admitted.
-End FDH.
-
-Theorem flatten_dec_full: forall stt d sol, ValidState stt -> WellFormedDecision d -> sol = flatten_decision stt d
-    -> Forall FullProba sol /\ exists x, In x sol.
+Lemma simplify_retrieve_wf : forall lst d,
+  WellFormedDecision d ->
+  WellFormedDecision (fold_right (fun (ic: item * nat) curdec => let (i, q) := ic in if 0 <? q then can_take i q curdec else curdec) d lst).
 Proof.
+  induction lst as [| [i q] lst IH]; intros d WFD.
+  - simpl. assumption.
+  - simpl. destruct (0 <? q) eqn:Hq.
+    + apply check_can_take.
+      * apply Nat.ltb_lt in Hq. Lia.lia.
+      * apply IH; auto.
+    + apply IH; auto.
+Qed.
+
+Lemma simplify_retrieve_cost : forall lst d,
+  (RHelpers.dec_amount 0
+    (fold_right (fun (ic: item * nat) curdec => let (i, q) := ic in if 0 <? q then can_take i q curdec else curdec) d lst)
+  <= list_sum (map snd lst) + length lst + RHelpers.dec_amount 0 d)%nat.
+Proof.
+  induction lst as [| [i q] lst IH]; intros d.
+  - simpl. Lia.lia.
+  - simpl. destruct (0 <? q) eqn:Hq; simpl; pose proof (IH d); Lia.lia.
+Qed.
+
+Theorem flatten_dec_full: forall stt d sol, 
+  ValidState stt -> WellFormedDecision d -> sol = flatten_decision stt d
+  -> Forall FullProba sol /\ exists x, In x sol.
+Proof.
+  intros stt d sol VS WFD Heq.
+  
+  (* Generalize our measure to use strong induction *)
+  remember (RHelpers.dec_amount (RHelpers.item_cost stt) d) as n.
+  generalize dependent stt. 
+  generalize dependent d. 
+  generalize dependent sol.
+  
+  (* Strong induction on the measure n *)
+  induction n as [n IHn] using lt_wf_ind.
+  intros sol d WFD stt VS Heq Hn.
+
+  destruct d;simp flatten_decision in Heq.
+
+  - (* App *) subst sol.
+    inversion WFD; subst.
+    assert (Forall FullProba (flatten_decision stt d1) /\ 
+            exists x, In x (flatten_decision stt d1)) as IH1.
+    {
+      (* We tell IHn what our smaller measure 'm' is *)
+      eapply (IHn (RHelpers.dec_amount (RHelpers.item_cost stt) d1)); try reflexivity; auto.
+      simpl. Lia.lia. 
+    }
+    assert (Forall FullProba (flatten_decision stt d2) /\ 
+            exists x, In x (flatten_decision stt d2)) as IH2.
+    {
+      eapply (IHn (RHelpers.dec_amount (RHelpers.item_cost stt) d2)); try reflexivity; auto.
+      simpl. Lia.lia.
+    }
+    destruct IH1 as [Hforall1 [x1 Hexists1]].
+    destruct IH2 as [Hforall2 [x2 Hexists2]].
+    split.
+    + apply Forall_app.
+      split; assumption.
+      
+    + exists x1.
+      apply in_app_iff.
+      left. assumption.
+  - (* retrieve equipment *) 
+    set (nstt := {| book := book stt; maxendurance := maxendurance stt; 
+                    curendurance := curendurance stt; sk := sk stt; 
+                    disciplines := disciplines stt; chapter := chapter stt; 
+                    items := items stt; flags := flags stt; previtems := empty |}) in *.
+    set (ndecision := RHelpers.simplify_retrieve_equipment stt d) in *.
+    eapply (IHn (RHelpers.dec_amount (RHelpers.item_cost nstt) ndecision)). 4: {
+      apply Heq.
+    }
+    + subst n.
+      unfold nstt. unfold RHelpers.item_cost at 1. simpl.
+      pose proof (simplify_retrieve_cost (previtems stt) d) as Hcost.
+      unfold RHelpers.item_cost.
+      unfold ndecision.
+      unfold RHelpers.simplify_retrieve_equipment.
+      Lia.lia.
+    + apply (simplify_retrieve_wf (previtems stt) d).
+      inversion WFD; subst. assumption.
+    + unfold nstt in *. subst. clear nstt.
+      destruct stt. unfold ValidState in *. simpl in *.
+      unfold ValidBag in VS.
+      repeat split; try tauto. constructor. constructor.
+    + reflexivity.
+  - (* can_take A *) 
+    subst sol.
+    inversion WFD; subst; clear WFD.
+    destruct n0; try Lia.lia.
+
+    assert (Forall FullProba (flatten_decision stt d) /\ 
+            exists x, In x (flatten_decision stt d)) as IH_notake.
+    {
+      eapply (IHn (RHelpers.dec_amount (RHelpers.item_cost stt) d)); try reflexivity; auto.
+      simpl. Lia.lia.
+    }
+    destruct IH_notake as [Hforall_notake [x_notake Hexists_notake]].
+    simpl in *.
+    destruct n0 as [| q']; simp flatten_decision; simpl.
+    + split.
+      * apply Forall_app.
+        split.
+        -- assumption.
+        -- apply Forall_forall.
+          intros x Hx.
+          apply in_flat_map in Hx.
+          destruct Hx as [nstt [Hnstt_in Hx_in]].
+           
+           (* Apply IHn to the inner call using the new state nstt *)
+          assert (Forall FullProba (flatten_decision (proj1_sig nstt) d) /\ 
+                   exists x, In x (flatten_decision (proj1_sig nstt) d)) as IH_nstt.
+          {
+            eapply (IHn (RHelpers.dec_amount (RHelpers.item_cost (proj1_sig nstt)) d)); try reflexivity; auto.
+            - destruct nstt as [stt' Heq_cost]. simpl in *. 
+              (* The item_cost is mathematically identical, so the measure decreases! *)
+              rewrite Heq_cost. Lia.lia.
+            - eapply RHelpers.get_wtakestts_valid; eauto.
+          }
+          destruct IH_nstt.
+          eapply Forall_forall in H; eauto.
+      * exists x_notake.
+        apply in_app_iff.
+        left.
+        exact Hexists_notake.
+    + split.
+      * apply Forall_app.
+        split; auto.
+        apply Forall_forall.
+        intros x Hx.
+        apply in_flat_map in Hx.
+        destruct Hx as [nstt [Hnstt_in Hx_in]].
+          assert (Forall FullProba (flatten_decision (proj1_sig nstt) (can_take i (S q') d)) /\ 
+                   exists x, In x (flatten_decision (proj1_sig nstt) (can_take i (S q') d))) as IH_nstt.
+          {
+            eapply (IHn (RHelpers.dec_amount (RHelpers.item_cost (proj1_sig nstt)) (can_take i (S q') d))); try reflexivity; auto.
+            - destruct nstt as [stt' Heq_cost]. simpl in *. 
+              (* The item_cost is mathematically identical, so the measure decreases! *)
+              rewrite Heq_cost. Lia.lia.
+            - constructor; auto. Lia.lia.
+            - eapply RHelpers.get_wtakestts_valid; eauto.
+          }
+          destruct IH_nstt.
+          eapply Forall_forall in H; eauto.
+      * exists x_notake.
+        apply in_app_iff.
+        left.
+        exact Hexists_notake.
+  - (* can_buy *)
+    inversion WFD; subst; clear WFD.
+    assert (Forall FullProba (flatten_decision stt d) /\ 
+            exists x, In x (flatten_decision stt d)) as IH_notake.
+    {
+      eapply (IHn (RHelpers.dec_amount (RHelpers.item_cost stt) d)); try reflexivity; auto.
+    }
+    destruct IH_notake as [Hforall_notake [x_notake Hexists_notake]].
+    simpl.
+    destruct (n0 <? sitems Gold stt).
+    + split.
+      * apply Forall_app.
+        split; auto.
+        apply Forall_forall.
+        intros x Hx.
+        apply in_flat_map in Hx.
+        destruct Hx as [nstt [Hnstt_in Hx_in]].
+        assert (Forall FullProba (flatten_decision (proj1_sig nstt) d) /\ 
+                  exists x, In x (flatten_decision (proj1_sig nstt) d)) as IH_nstt.
+        {
+          eapply (IHn (RHelpers.dec_amount (RHelpers.item_cost (proj1_sig nstt)) d)); try reflexivity; auto.
+          - destruct nstt as [stt' Heq_cost]. simpl in *. 
+            rewrite Heq_cost.
+            assert (RHelpers.item_cost (c_rm_items Gold n0 stt) = RHelpers.item_cost stt). {
+              apply RHelpers.update_stt_preserve_cost.
+              unfold c_rm_items, update_endurance; simpl.
+              reflexivity.
+            }
+            rewrite H.
+            Lia.lia.
+          - eapply RHelpers.get_wtakestts_valid; eauto.
+          - eapply RHelpers.get_wtakestts_valid; eauto.
+        }
+        
+    split.
+  - (* can_sell *)
+    inversion WFD; subst; clear WFD.
+    admit.
+  - (* conditional *)
+    inversion WFD; subst; clear WFD.
+    admit.
+  - (* special *)
+    inversion WFD; subst; clear WFD.
+    admit.
+  - (* none *)
+    inversion WFD; subst; clear WFD.
+    admit.
+  - (* evade_fight *)
+    inversion WFD; subst; clear WFD.
+    admit.
+  - (* after_combat *)
+    inversion WFD; subst; clear WFD.
+    admit.
+  - (* remove_item_from *)
+    inversion WFD; subst; clear WFD.
+    admit.
 Admitted.
 
-
-(*
-Theorem rules_are_preserving_fullproba: forall stt co fuel sol, ValidState stt -> WellFormedCO co ->
-         sol = s_update_d fuel stt co ->
-          FullProba sol.
-Proof.
-  intros stt co fuel sol VS WCO EQC.
-  subst.
-  generalize dependent stt.
-  generalize dependent fuel.
-  induction WCO; intros; destruct fuel; simpl; repeat RHelpers.rap; auto.
-  * apply (H0 b c); auto.
-    pose proof (incl_filter (fun kv: bool_cond * chapter_outcome => check_cond stt (fst kv)) lst) as Hincl.
-    rewrite Heql in Hincl.
-    apply incl_cons_inv in Hincl. tauto.
-
-  * pose proof (RHelpers.in_map_fst x lst). apply H3 in H2. destruct H2.
-    eapply H1; eauto.
-
-  * unfold fight.
-    destruct (Modifiers.ValidMods_dec l) eqn: VM; try contradiction.
-    remember (f_fight stt s e l v).
-    symmetry in Heqp.
-    apply fight_inductive in Heqp.
-    eapply ifight_correct; eauto.
-  
-  * destruct x; inversion Heqp; subst; clear Heqp; destruct (has_mod MultiFight l) eqn:MF; try apply RHelpers.goto_fullmap.
-    + apply IHWCO.
-      repeat RHelpers.rap.
-      apply Insert.insert_with_valid; auto.
-    + apply IHWCO.
-      repeat RHelpers.rap.
-      apply Delete.valid.
-      apply Delete.valid.
-      assumption.
-      apply Insert.insert_with_valid; auto.
-  
-  * remember (fight stt s e l) as res.
-    pose proof (fight_res_hp stt s e l res) as FRH.
-    lapply FRH; auto; intro FRH2; clear FRH.
-    simpl in H.
-    symmetry in Heqres.
-    specialize (FRH2 H Heqres).
-    subst.
-    eapply Forall_forall in H0; try apply FRH2.
-    unfold valid_fight_result in H0.
-  
-    destruct x; inversion Heqp; subst; clear Heqp; destruct (has_mod MultiFight l) eqn:MF; try apply RHelpers.goto_fullmap.
-    + eapply IHWCO.
-      apply VS.update_endurance.
-      { 
-        intros. simpl. split; try Lia.lia.
-        rewrite MH.update_flags.
-        assumption.
-      }
-      apply VS.update_flags; auto.
-      intros.
-      apply Insert.insert_with_valid; auto.
-    + eapply IHWCO.
-      apply VS.update_endurance.
-      { intros. simpl. rewrite MH.update_flags. rewrite MH.update_flags. Lia.lia. }
-      apply VS.update_flags; auto.
-      intros.
-      apply Delete.valid.
-      apply Delete.valid.
-      assumption.
-      apply VS.update_flags; auto.
-      intros.
-      apply Insert.insert_with_valid; auto.
-  
-  * apply fight_round_full.
-  * unfold FullProba.
-    subst.
-    remember (fight_round stt s e l) as fr.
-    symmetry in Heqfr.
-    pose proof (FRH.fight_round_vr stt s e l fr Heqfr).
-    pose proof (Merge.use_forall _ _ _ H1 H0). simpl in H2.
-    remember (NatLemma.nat_cmp (curendurance stt - S n) (e - n0)) as xc.
-    unfold ValidState in VS. simpl in VS.
-
-    destruct xc; try apply IHWCO1; try apply IHWCO2; try apply IHWCO3;
-      apply VS.update_endurance; intros; simpl; try Lia.lia;
-      try apply VS.update_flags; try assumption; intros;
-      try apply Insert.insert_with_valid;
-      try apply Delete.valid;
-      try apply Delete.valid;
-      try assumption;
-      rewrite MH.update_flags;
-      split;
-      try Lia.lia
-      .
-
-  * admit.
-  * admit.
-  * destruct q; try Lia.lia.
-    unfold FullProba.
-    rewrite merge_proba_rebuild_full.
-    apply RHelpers.lose_items_full.
-    intros.
-    apply IHWCO.
-    Search (merge_probas).
-*)
+End FlattenDec.
